WIP Prove trivial_init, trivial_sim

coq/exec/Nop.v
@@ -257,229 +257,71 @@ Proof.
   apply H0 in H.
   inv H.
 Qed.
-(* sim_local : *)
-(* Config -> *)
-(* Config -> ECStack -> ECStack -> Relational.t -> nat -> State -> State -> Prop *)
-
-(* Argument scopes are [_ _ _ _ _ nat_scope _ _] *)
-(* sim_local is transparent *)
-(* Expands to: Constant LLVMBerry.exec.SimulationLocal.sim_local *)
-
-
-(* _sim_local : *)
-(* Config -> *)
-(* Config -> *)
-(* (ECStack -> ECStack -> Relational.t -> nat -> State -> State -> Prop) -> *)
-(* ECStack -> ECStack -> Relational.t -> nat -> State -> State -> Prop *)
-
-(* Argument scopes are [_ _ _ _ _ _ nat_scope _ _] *)
-(* Expands to: Inductive LLVMBerry.exec.SimulationLocal._sim_local *)
-
-
-(* nop_state_sim : *)
-(* ECStack -> ECStack -> Relational.t -> nat -> State -> State -> Prop *)
-
-(* Argument scopes are [_ _ _ nat_scope _ _] *)
-(* Expands to: Inductive Top.nop_state_sim *)
-
 
 Inductive trivial_state_sim (stack0_src stack0_tgt : ECStack) (inv : Relational.t)
           : nat -> State -> State -> Prop :=
   trivial_state_sim_intro :
-    forall same_state
-      (SRC_STACK : ECS same_state = stack0_src)
-      (TGT_STACK : ECS same_state = stack0_tgt),
+    forall state_src state_tgt
+      (SRC_STACK : ECS state_src = stack0_src)
+      (TGT_STACK : ECS state_tgt = stack0_tgt),
     trivial_state_sim stack0_src stack0_tgt inv
-                      (length (CurCmds (EC same_state)))
-                      same_state same_state.
+                      (length (CurCmds (EC state_tgt)))
+                      state_src state_tgt.
 
 Lemma trivial_step
       conf_src conf_tgt:
   trivial_state_sim <6= (sim_local conf_src conf_tgt).
+Admitted.
+
+Lemma trivial_init
+      conf_src conf_tgt
+      stack_src stack_tgt
+      mem_src mem_tgt
+      same_fdef
+      args_src args_tgt
+      inv
+      ec_tgt
+      (ARGS: list_forall2 (GVs.inject inv.(Relational.alpha)) args_src args_tgt)
+      (INIT: init_fdef conf_tgt same_fdef args_tgt ec_tgt):
+  exists ec_src idx,
+    init_fdef conf_src same_fdef args_src ec_src /\
+    trivial_state_sim
+      stack_src stack_tgt
+      inv idx
+      (mkState ec_src stack_src mem_src)
+      (mkState ec_tgt stack_tgt mem_tgt).
 Proof.
-  pcofix CIH. i.
-  inv PR.
-  pfold; simpl.
- 
-  destruct x5. (* eqn:T. *)
-  destruct EC0. (* eqn:T2. *)
-  destruct CurCmds0. (* eqn:T3. *)
-  destruct conf_tgt, conf_src.
-  -
-    destruct Terminator0. (* eqn:T4. *)
-    + (* insn_return *)
-      eapply _sim_local_return; repeat (simpl; eauto).
-      admit. admit. admit.
-    + (* insn_return_void *)
-      eapply _sim_local_return_void; repeat (simpl; eauto).
-    + (* insn_br *)
-      eapply _sim_local_step; repeat (simpl; eauto).
-      unfold stuck_state, not.
-      apply double_neg2.
-      repeat eexists.
-      eapply sBranch; simpl; eauto.
-      admit. admit. admit.
+  inv INIT.
+  do 2 eexists.
+  splits.
+  econs; eauto. erewrite locals_init; eauto.
+  eapply trivial_state_sim_intro; eauto.
+Qed.
 
-      ii.
-      destruct event.
-      *
-        inv STEP.
-        eexists.
-        eexists.
-        eexists.
-        eexists.
-        eexists.
-        splits.
-        econs; simpl; eauto.
-        econs; simpl; eauto.
-        eapply sBranch; simpl; eauto.
-        admit. admit. admit.
-        econs; simpl; eauto.
-
-        pfold; simpl.
-    +
-      
-        | _sim_local_return : forall (st2_src : State) (id2_src : id)
-                          (typ2_src : typ) (ret2_src : value) 
-                          (id1_tgt : id) (typ1_tgt : typ) 
-                          (ret1_tgt : value)
-                          (retval2_src retval1_tgt : GenericValue),
-                        sop_star conf_src st1_src st2_src events.E0 ->
-                        CurCmds (EC st2_src) = [] ->
-                        CurCmds (EC st1_tgt) = [] ->
-                        Terminator (EC st2_src) =
-                        insn_return id2_src typ2_src ret2_src ->
-                        Terminator (EC st1_tgt) =
-                        insn_return id1_tgt typ1_tgt ret1_tgt ->
-                        typ2_src = typ1_tgt ->
-                        ECS st2_src = stack0_src ->
-                        ECS st1_tgt = stack0_tgt ->
-                        True ->
-                        getOperandValue (CurTargetData conf_src) ret2_src
-                          (Locals (EC st2_src)) (Globals conf_src) =
-                        Some retval2_src ->
-                        getOperandValue (CurTargetData conf_tgt) ret1_tgt
-                          (Locals (EC st1_tgt)) (Globals conf_tgt) =
-                        Some retval1_tgt ->
-                        GVs.inject (Relational.alpha inv1) retval2_src
-                          retval1_tgt ->
-                        _sim_local conf_src conf_tgt sim_local stack0_src
-                          stack0_tgt inv1 idx1 st1_src st1_tgt
-
-                          ECS0 = x0
-                                   subgoal 2 (ID 1106) is:
-                          ECS0 = x1
-
-
-    +
-    econs; simpl; eauto.
-    unfold stuck_state, not; i.
-    inv H.
-    inv H0.
-    inv H.
-    (* (sInsn_cases (inversion H) Case). *)
-  -
-  eapply _sim_local_step; simpl; eauto.
-  unfold stuck_state, not.
-  apply double_neg2.
-
-  repeat eexists.
-
+Lemma trivial_sim
+      conf_src conf_tgt
+      fdef_same :
+  sim_func conf_src conf_tgt fdef_same fdef_same.
+Proof.
+  ii.
+  exploit trivial_init; eauto.
+  ii.
+  inv x0. inv H. inv H0. inv H1.
+  do 2 eexists.
+  splits; eauto.
+  apply trivial_step.
+  eapply trivial_state_sim_intro; simpl; eauto.
+  
+  Unshelve.
+  apply mem0_tgt.
+  apply mem0_src.
+Qed.
 
 Lemma nop_step
       conf_src conf_tgt:
   nop_state_sim <6= (sim_local conf_src conf_tgt).
 Proof.
-  pcofix CIH. i.
-  inv PR.
-  pfold; simpl.
-  
-  (* destruct (cmds_src) eqn:EMPTY_CMD. *)
-  (* - (* empty_src *) *)
-  (*   subst; simpl. *)
-  (*   destruct (cmds_tgt) eqn:EMPTY_TGT. *)
-  (*   + *)
-  (*     destruct term. *)
-  (*     * *)
-  (*       eapply _sim_local_return; simpl; eauto. *)
-  (*       simpl; eauto. *)
-  (*       simpl; eauto. *)
-  (*       admit. *)
-  (*       admit. *)
-  (*       admit. *)
-  (*     * *)
-  (*       (* return_void *) *)
-  (*       eapply _sim_local_return_void; simpl; eauto. *)
-  (*       simpl; eauto. *)
-  (*     * *)
-  (*       (* insn_br *) *)
-  (*       destruct conf_tgt. *)
-  (*       destruct value5. *)
-  (*       eapply _sim_local_step; simpl; eauto. *)
-  (*       unfold stuck_state, not. *)
-  (*       apply double_neg2. *)
-  (*       repeat eexists. *)
-  (*       eapply sBranch; simpl; eauto. *)
-  (*       admit. *)
-  (*       admit. *)
-  (*       admit. *)
-
-  (*       admit. *)
-  (*       admit. *)
-  (*     * (* insn_br_uncond *) *)
-  (*       admit. *)
-  (*     * (* insn_unreachable *) *)
-  (*       admit. *)
-  (*   + *)
-  (* - *)
-  
-  destruct (forallb is_nop cmds_tgt) eqn:ALL_NOP.
-  -
-    assert(G:(forallb is_nop cmds_src)) by admit.
-    destruct cmds_src eqn:SRC_EMPTY;
-      destruct cmds_tgt eqn:TGT_EMPTY;
-      subst; simpl.
-    +
-      destruct term.
-      *
-        (* return *)
-        destruct value5;
-        eapply _sim_local_return; simpl; eauto; unfold Terminator; simpl; eauto.
-        admit.
-        admit.
-        admit.
-        admit.
-        admit.
-        admit.
-      *
-        (* return_void *)
-        eapply _sim_local_return_void; simpl; eauto; unfold Terminator; simpl; eauto.
-      *
-        (* br *)
-        admit.
-      *
-        destruct conf_tgt, conf_src.
-        
-        eapply _sim_local_step; simpl; eauto.
-        apply double_neg2.
-        repeat eexists.
-        eapply sBranch_uncond; simpl; eauto.
-        admit. (* <___________________ not able *)
-        admit.
-
-        intros.
-        repeat eexists.
-        eapply sop_star_nil; simpl; eauto.
-        econs; eauto.
-        instantiate (1:=st3_tgt).
-        eapply sBranch_uncond.
-      *
-        (* br_uncond *)
-        *
-        (* br_unreachable *)
-  -
-    
-    
+Qed.
 
 Lemma nop_sim
       conf_src conf_tgt
